kosaraju-lean4/Graph/Scc.lean
@@ -1,0 +1,161 @@
+import Graph.DirectedGraph
+
+def in_same_scc [DirectedGraph V Graph]
+                [BEq V] [LawfulBEq V]
+                (g : Graph)
+                (a b : V)
+                : Prop := reachable g a b /\ reachable g b a
+
+theorem same_scc_trans [DirectedGraph V Graph]
+                       [BEq V] [LawfulBEq V]
+                       (g : Graph)
+                       (x y z : V) :
+in_same_scc g x y -> in_same_scc g y z -> in_same_scc g x z := by
+simp [in_same_scc]
+intros
+constructor
+all_goals apply reachable_trans
+all_goals assumption
+
+def is_subscc [DirectedGraph V Graph]
+              [BEq V] [LawfulBEq V]
+              (g : Graph)
+              (s : Finset V) : Prop :=
+    ∀ x y, x ∈ s -> y ∈ s -> in_same_scc g x y
+
+def is_scc [DirectedGraph V Graph]
+           [BEq V] [LawfulBEq V]
+           (g : Graph)
+           (s : Finset V) : Prop :=
+    is_subscc g s /\ (∀ s', s ⊆ s' -> is_subscc g s' -> s' ⊆ s)
+
+theorem in_same_scc_transpose [DirectedGraph V Graph]
+                              [BEq V] [LawfulBEq V]
+                              (g : Graph)
+                              (a b : V) :
+in_same_scc (DirectedGraph.transpose V g) a b <-> in_same_scc g a b := by
+simp [in_same_scc]
+repeat rw [reachable_transpose]
+tauto
+
+theorem is_subscc_transpose [DirectedGraph V Graph]
+                            [BEq V] [LawfulBEq V]
+                            (g : Graph)
+                            (cc : Finset V) :
+is_subscc g cc <-> is_subscc (DirectedGraph.transpose V g) cc := by
+simp [is_subscc]
+constructor
+all_goals intros h x y
+all_goals specialize h x y
+all_goals rw [in_same_scc_transpose] at *
+all_goals tauto
+
+private theorem is_scc_transpose_inner [DirectedGraph V Graph]
+                                       [BEq V] [LawfulBEq V]
+                                       (g : Graph)
+                                       (cc : Finset V) :
+is_scc g cc -> is_scc (DirectedGraph.transpose V g) cc := by
+simp [is_scc]
+intros
+rw [<- is_subscc_transpose]
+simp_all
+intros
+rw [<- is_subscc_transpose] at *
+tauto
+
+theorem is_scc_transpose [DirectedGraph V Graph]
+                          [BEq V] [LawfulBEq V]
+                          (g : Graph)
+                          (cc : Finset V) :
+is_scc g cc <-> is_scc (DirectedGraph.transpose V g) cc := by
+constructor
+. exact is_scc_transpose_inner g cc
+. intros h
+  have h := is_scc_transpose_inner _ _ h
+  rw [DirectedGraph.transpose_transpose] at h
+  assumption
+
+theorem scc_max [DirectedGraph V Graph]
+                [BEq V] [LawfulBEq V] [DecidableEq V]
+                (g : Graph)
+                (x y : V) (cc : Finset V)
+                (h₁ : is_scc g cc)
+                (h₃ : x ∈ cc)
+                (h₄ : in_same_scc g x y) : y ∈ cc := by
+simp [is_scc] at *
+obtain ⟨h₁, h₂⟩ := h₁
+
+have h₅ : ∀ z ∈ cc, in_same_scc g z y := by
+  intros z h₅
+  specialize h₁ x z h₃ h₅
+  apply same_scc_trans <;> try assumption
+  simp [in_same_scc] at *; tauto
+
+have : is_subscc g (insert y cc) := by
+  intros a b h₆ h₇
+  simp_all
+  cases h₇ <;> cases h₆ <;> try tauto
+  all_goals subst y
+  . subst b
+    specialize h₅ x h₃
+    obtain ⟨h₅, _ ⟩ := h₅
+    have := reachable_valid _ _ _ h₅
+    constructor
+    all_goals right
+    all_goals simp_all
+  . apply h₅; assumption
+  . specialize h₅ b
+    simp [in_same_scc] at *
+    simp_all
+
+apply h₂ (insert y cc) <;> simp_all
+
+
+theorem disjoint_scc [DirectedGraph V Graph]
+                     [BEq V] [LawfulBEq V] [DecidableEq V]
+                     (g : Graph)
+                     (cc1 cc2 : Finset V)
+                     (h₁ : Nonempty (cc1 ∩ cc2 : Finset V))
+                     (h₂ : is_scc g cc1)
+                     (h₄ : is_scc g cc2) :
+                     cc1 = cc2 := by
+obtain ⟨x, h₁⟩ := h₁
+apply Finset.Subset.antisymm
+all_goals intros y h₉
+all_goals have h₈ : x = y \/ ¬ x = y := by tauto
+all_goals cases h₈
+any_goals simp_all
+all_goals apply scc_max g x y
+any_goals assumption
+any_goals tauto
+. obtain ⟨h₂, _⟩ := h₂
+  apply h₂ <;> tauto
+. obtain ⟨h₄, _⟩ := h₄
+  apply h₄ <;> tauto
+
+theorem scc_navel [DirectedGraph V Graph]
+                  [BEq V] [LawfulBEq V] [DecidableEq V]
+                  {g : Graph}
+                  {cc : Finset V}
+                  (x : V)
+                  (h₂ : ∀ y ∈ cc, reachable g y x)
+                  (h₁ : ∀ y ∈ cc, reachable g x y) :
+is_subscc g cc := by
+intros a b ha hb
+constructor
+. apply reachable_trans g a x b
+  . apply h₂ ; assumption
+  . apply h₁ ; assumption
+. apply reachable_trans g b x a
+  . apply h₂ ; assumption
+  . apply h₁ ; assumption
+
+structure Trajectory (Graph V : Type*)
+                     [DirectedGraph V Graph]
+                     [BEq V] [LawfulBEq V] [DecidableEq V]
+                     (graph: Graph)
+where
+  sccs_o  : List (Finset V)
+  p₂ : ∀ cc, cc ∈ sccs_o ↔ Nonempty cc /\ is_scc graph cc /\ ∀ x ∈ cc, x ∈ DirectedGraph.vertices graph
+  p₄ : ∀ cc₁ ∈ sccs_o, ∀ cc₂ ∈ sccs_o, cc₁ = cc₂ \/ cc₁ ∩ cc₂ = Finset.empty
+  p₅ : ∀ v ∈ DirectedGraph.vertices graph, ∃ cc, v ∈ cc /\ cc ∈ sccs_o
