kosaraju-lean4/Kosaraju.lean
@@ -1,4 +1,5 @@
 -- This module serves as the root of the `Kosaraju` library.
 -- Import modules here that should be built as part of the library.
+import «Graph».AdjacencyTable
 import «Kosaraju».Basic
-import «Kosaraju».AdjacencyTable
+import «Tarjan».Basic
