kosaraju-lean4/Kosaraju/Dfs2.lean
@@ -1,8 +1,9 @@
-import Kosaraju.DirectedGraph
+import Graph.DirectedGraph
+import Graph.Scc
+import Graph.ReachableBefore
+import ListHelper.Rank
 import Mathlib.Tactic.Tauto
 import Std.Data.List.Lemmas
-
-open Rank
 
 structure Funnel [DirectedGraph V Graph] [BEq V] [LawfulBEq V]
                   (graph: Graph)
@@ -16,8 +17,8 @@ where
 def dfs2 [DirectedGraph V Graph] [BEq V] [LawfulBEq V]
          (graph: Graph)
          (roots black_stack grays : List V)
-         (h₁: roots ⊆ DirectedGraph.all_nodes graph)
-         (h₂: grays ⊆ DirectedGraph.all_nodes graph)
+         (h₁: roots ⊆ DirectedGraph.vertices graph)
+         (h₂: grays ⊆ DirectedGraph.vertices graph)
          (h₃: wff_color graph black_stack grays)
          : Funnel graph roots black_stack grays := match roots with
 | List.nil => {
@@ -70,7 +71,7 @@ def dfs2 [DirectedGraph V Graph] [BEq V] [LawfulBEq V]
                     . rw [simplelist_tl]
                       simp_all
                       tauto
-    let v : List V := (DirectedGraph.all_nodes graph)
+    let v : List V := (DirectedGraph.vertices graph)
     let termination_proof: grays.length < v.length := by
       apply simplelist_size_2
       . tauto
@@ -109,15 +110,6 @@ def dfs2 [DirectedGraph V Graph] [BEq V] [LawfulBEq V]
       obtain ⟨_, ⟨h₃, _⟩⟩ := h₃
       specialize h₃ _ _ h₄ h₂
       cases h₃
-      . have h₆: simplelist (List.cons x stack) := by
-          rw [simplelist_tl]
-          constructor <;> try assumption
-          simp [wff_color, reachable_before_same_scc] at *
-          tauto
-        specialize h₆ b
-        rw [h, num_occ_concat] at h₆
-        rw [mem_num_occ] at *
-        omega
       . obtain ⟨s', _, _⟩ := monotony
         subst stack
         simp [wff_color, reachable_before_same_scc] at p₃
@@ -133,6 +125,15 @@ def dfs2 [DirectedGraph V Graph] [BEq V] [LawfulBEq V]
           apply g
           tauto
         . tauto
+      . have h₆: simplelist (List.cons x stack) := by
+          rw [simplelist_tl]
+          constructor <;> try assumption
+          simp [wff_color, reachable_before_same_scc] at *
+          tauto
+        specialize h₆ b
+        rw [h, num_occ_concat] at h₆
+        rw [mem_num_occ] at *
+        omega
     have g₉: no_path_out_of_in graph black_stack (List.cons x stack) := by
       apply no_edge_out_of_no_path_out_of_in ; assumption
     have h₆ := by
@@ -186,5 +187,5 @@ def dfs2 [DirectedGraph V Graph] [BEq V] [LawfulBEq V]
                                                   subst a
                                                   tauto
     }
-termination_by let v : List V := DirectedGraph.all_nodes graph
+termination_by let v : List V := DirectedGraph.vertices graph
                (v.length - grays.length, roots)
