kosaraju-lean4/ListHelper/Rip.lean
@@ -1,0 +1,27 @@
+import Mathlib.Tactic.Tauto
+
+structure Rapport (x : V) (s : List V) where
+  s1 : List V
+  last : x ∈ s -> ∃ s2, s1 ++ x :: s2 = s
+
+def split_once [DecidableEq V] (x : V) (s: List V) : Rapport x s := match s with
+| [] => {
+          s1 := []
+          last := by tauto
+        }
+| y :: s => if dite : x = y then
+              {
+                s1 := []
+                last := by tauto
+              }
+            else
+              let ⟨s1, last⟩ := split_once x s
+              {
+                s1 := y :: s1
+                last := by intros h
+                           cases h
+                           . tauto
+                           . obtain ⟨s3, h⟩ := last (by tauto)
+                             subst s
+                             exists s3
+              }
