kosaraju-lean4/ListHelper/Union.lean
@@ -1,0 +1,39 @@
+import Mathlib.Data.Finset.Basic
+open Finset
+
+theorem pertinent
+[BEq V] [LawfulBEq V] [DecidableEq V]
+{sccs : List (Finset V)} :
+∀ (init : Finset V),
+List.foldl Union.union init sccs = init ∪ List.foldl Union.union ∅ sccs
+:= by
+induction sccs <;> simp
+rename_i scc sccs induction_step
+intros
+rw [induction_step, induction_step scc]
+simp
+
+theorem union_helper
+[BEq V] [LawfulBEq V] [DecidableEq V]
+{x : V} {sccs : List (Finset V)} :
+x ∈ List.foldl Union.union ∅ sccs ↔ (∃ cc, x ∈ cc /\ cc ∈ sccs) := by
+induction sccs
+. tauto
+. simp
+  rw [pertinent]
+  simp
+  rename_i h
+  rw [h]
+  constructor <;> intros h <;> cases h
+  . tauto
+  . rename_i h
+    obtain ⟨cc, h⟩ := h
+    use cc
+    tauto
+  . rename_i h
+    obtain ⟨_, h⟩ := h
+    cases h
+    . rename_i h
+      rw [<- h]
+      tauto
+    . tauto
