kosaraju-lean4/Tarjan/Basic.lean
@@ -1,0 +1,67 @@
+import Tarjan.Env
+import Tarjan.Dfs
+
+def tarjan [DirectedGraph V Graph]
+           [BEq V] [LawfulBEq V] [DecidableEq V]
+           (graph: Graph) : Trajectory Graph V graph :=
+let e : Env V graph := {
+  black := ∅
+  gray := ∅
+  stack := []
+  sccs := []
+  num := fun _ => -1
+  num_clamp := by tauto
+  num_1 := by tauto
+  num_infty := by tauto
+  valid_gray  := by tauto
+  valid_black := by tauto
+  disjoint_gb := by tauto
+  color := by tauto
+  stack_finset := by tauto
+  simplelist_stack := by tauto
+  decreasing_stack := by tauto
+  wf_stack₂ := by tauto
+  wf_stack₃ := by tauto
+  sccs_in_black := by simp
+                      intros _ x h h₁ _
+                      specialize h₁ h
+                      tauto
+  sccs_disjoint := by simp
+}
+let ⟨n, e', p₁, p₃, p₄, p₅, p₆⟩ := dfs graph (DirectedGraph.vertices graph) e (by tauto) (by tauto)
+have empty_gray  : e'.gray  = ∅ := by rw [← p₁.eq_gray]
+have empty_stack : e'.stack = [] := by
+  have h : e'.stack = [] \/ ∃ x xs, e'.stack = x :: xs := by cases e'.stack <;> tauto
+  cases h with
+  | inl h => tauto
+  | inr h => obtain ⟨x, xs, h⟩ := h
+             have h₁ := e'.wf_stack₃ x
+             rw [h, empty_gray] at h₁
+             tauto
+have eq_black : ∀ x, x ∈ DirectedGraph.vertices graph ↔ x ∈ e'.black := by
+  intros x
+  constructor
+  . specialize p₃ x
+    rw [empty_gray] at p₃
+    simp at p₃
+    tauto
+  . apply e'.valid_black
+{
+  sccs_o := e'.sccs
+  p₂ := by intros cc
+           rw [e'.sccs_in_black]
+           constructor <;> intros h <;> simp_all
+           . intros x hx
+             obtain ⟨_, h, _⟩ := h
+             apply h hx
+           . obtain ⟨_, _, h⟩ := h
+             exact h
+  p₄ := e'.sccs_disjoint
+  p₅ := by simp [num_of_reachable] at p₅
+           have h := shrewd e'
+           rw [empty_gray, empty_stack] at h
+           simp at h
+           intro x
+           rw [eq_black, h, union_helper]
+           tauto
+}
