kosaraju-lean4/Tarjan/Dfs.lean
@@ -1,0 +1,1010 @@
+import Graph.DirectedGraph
+import ListHelper.Rip
+import ListHelper.Union
+import Mathlib.Data.Finset.Basic
+import Mathlib.Data.Finset.Card
+import Std.Data.List.Lemmas
+import Tarjan.Env
+
+open Finset
+open Finset List
+
+set_option maxHeartbeats 0
+
+structure Flair [DirectedGraph V Graph]
+                [BEq V] [LawfulBEq V] [DecidableEq V]
+                (graph : Graph) (x : V) (e : Env V graph)
+where
+n : Int
+e' : Env V graph
+p₁ : SubEnv e e'
+p₃ : x ∈ e'.black
+p₄ : n ≤ e'.num x
+p₅ : let infty : Int := (DirectedGraph.vertices graph: List V).length
+     n = infty \/ num_of_reachable n x e'
+p₆ : ∀ y ∈ e.stack, (∃ s, e'.stack = s ++ e.stack /\ ∃ x ∈ s, DirectedGraph.edge graph x y) → n ≤ e'.num y
+
+structure Shuttle [DirectedGraph V Graph]
+                  [BEq V] [LawfulBEq V] [DecidableEq V]
+                  (graph : Graph) (roots: List V) (e : Env V graph)
+where
+n : Int
+e' : Env V graph
+p₁ : SubEnv e e'
+p₃ : ∀ y ∈ roots, y ∈ e'.gray ∪ e'.black
+p₄ : ∀ y ∈ roots, n ≤ e'.num y
+p₅ : let infty : Int := (DirectedGraph.vertices graph: List V).length
+     n = infty \/ ∃ x ∈ roots, num_of_reachable n x e'
+p₆ : ∀ y ∈ e.stack, (∃ s, e'.stack = s ++ e.stack /\ ∃ x ∈ s, DirectedGraph.edge graph x y) → n ≤ e'.num y
+
+mutual
+
+def dfs3 [DirectedGraph V Graph]
+         [BEq V] [LawfulBEq V] [DecidableEq V]
+         (graph : Graph) (x : V) (e : Env V graph)
+         (a₁ : x ∈ DirectedGraph.vertices graph)
+         (a₂ : access_to graph e.gray x)
+         (a₃ : ¬ x ∈ e.gray)
+         (a₄ : ¬ x ∈ e.black)
+         : Flair graph x e :=
+-- let n0 := e.gray.card + e.black.card
+have h := by intros y hy z hz
+             rw [DirectedGraph.edge_succ] at hy
+             simp [add_stack_incr] at hz
+             cases hz with
+             | inl _ => subst z; tauto
+             | inr hz => specialize a₂ z hz
+                         apply reachable_trans graph z x y a₂
+                         tauto
+have : ¬ x ∈ e.stack := by
+  intros h
+  rw [e.stack_finset] at h
+  simp at h
+  tauto
+have h₁ : e.gray ∪ e.black ⊆ toFinset (DirectedGraph.vertices graph) := by
+  intros y h
+  simp at h
+  cases h <;> simp_all
+  . apply e.valid_gray; assumption
+  . apply e.valid_black; assumption
+
+have h₂ : Insert.insert x (e.gray ∪ e.black) ⊆ toFinset (DirectedGraph.vertices graph) := by
+  intros y h
+  simp at h
+  cases h <;> simp_all
+  rename_i h
+  cases h
+  . apply e.valid_gray; assumption
+  . apply e.valid_black; assumption
+
+have termination_proof : (toFinset (DirectedGraph.vertices graph) \
+  ((add_stack_incr e x a₁ a₂ a₃ a₄).gray ∪ (add_stack_incr e x a₁ a₂ a₃ a₄).black)).card <
+  (toFinset (DirectedGraph.vertices graph) \ (e.gray ∪ e.black)).card := by
+  rw [Finset.card_sdiff]
+  rw [Finset.card_sdiff]
+  any_goals simp [add_stack_incr]
+  any_goals assumption
+  . have h := Finset.card_le_card h₂
+    rw [card_insert_of_not_mem] at *
+    . omega
+    . intros h; simp at h; cases h <;> tauto
+    . intros h; simp at h; cases h <;> tauto
+
+
+let ⟨n1, e1, p₁, p₃, p₄, p₅, p₆⟩ := dfs graph (DirectedGraph.succ graph x) (add_stack_incr e x a₁ a₂ a₃ a₄) (by apply succ_valid; assumption) h
+have : x ∈ e1.gray := by
+  rw [<- p₁.eq_gray]
+  simp [add_stack_incr]
+have not_x_in_black : ¬ x ∈ e1.black := by
+  intros _
+  have hb : {x} ≤ e1.black := by simp; assumption
+  have hg : {x} ≤ e1.gray := by simp; assumption
+  have h := e1.disjoint_gb hg hb
+  simp at h
+have h₈ : e1.num x = e.gray.card + e.black.card := by
+  rw [<- p₁.stack_num]
+  all_goals simp [add_stack_incr]
+let ⟨s, last⟩ := split_once x e1.stack
+have h₇ : s ++ x :: e.stack = e1.stack /\ ∀ y ∈ s, y ∈ e1.black := by
+  obtain ⟨s, h, h₁⟩ := p₁.sub_stack
+  simp [add_stack_incr] at h h₁
+  obtain ⟨s3, h₂⟩ := last (by apply gray_le_stack; assumption)
+  have h₃ := e1.simplelist_stack
+  rw [h] at h₂ h₃
+  symm at h₂
+  obtain ⟨_, _⟩ := simplelist_uniq _ _ _ _ h₂ h₃
+  subst s3 s
+  tauto
+if dite : n1 < e.gray.card + e.black.card then
+  have p₅ : ∃ y ∈ DirectedGraph.succ graph x, ∃ z ∈ e1.stack, n1 = e1.num z ∧ reachable graph y z := by
+    cases p₅ <;> try tauto
+    subst n1
+    have := sn_bound e
+    omega
+  have : erase e1.gray x ∪ insert x e1.black ⊆ e1.gray ∪ e1.black := by
+    intros y h
+    have hy : y = x \/ ¬ y = x := by tauto
+    cases hy <;> simp_all
+  have : e1.gray ∪ e1.black ⊆ erase e1.gray x ∪ insert x e1.black := by
+    intros y h
+    have hy : y = x \/ ¬ y = x := by tauto
+    cases hy <;> simp_all
+  have h₉ : erase e1.gray x ∪ insert x e1.black = e1.gray ∪ e1.black := by
+    apply Finset.Subset.antisymm <;> assumption
+  have disjoint_gb : Disjoint (erase e1.gray x) (insert x e1.black) := by
+    simp
+    rw [Finset.erase_eq e1.gray x]
+    apply Disjoint.disjoint_sdiff_left e1.disjoint_gb
+  have h₆ : ∃ y ∈ e1.gray, e1.num y < e1.num x /\ in_same_scc graph x y := by
+    obtain ⟨y, p₅, z, h, h₁, h₂⟩ := p₅
+    obtain ⟨k, h₃, h₄, h₅⟩ := e1.wf_stack₃ z h
+    use k
+    have : e1.num z < e1.num x := by rw [<- h₁]; omega
+    have : e1.num k < e1.num x := by omega
+    repeat any_goals apply And.intro
+    any_goals assumption
+    . apply reachable_trans _ x z k
+      any_goals assumption
+      apply reachable_trans _ x y z
+      any_goals assumption
+      rw [DirectedGraph.edge_succ] at p₅
+      tauto
+    . apply e1.wf_stack₂
+      any_goals omega
+      any_goals apply gray_le_stack
+      all_goals assumption
+  {
+    n := n1
+    e' := {
+black := insert x e1.black
+gray := erase e1.gray x
+stack := e1.stack
+sccs := e1.sccs
+num := e1.num
+num_clamp := by
+  intros y
+  have h := Finset.card_union_of_disjoint disjoint_gb
+  rw [h₉, Finset.card_union_of_disjoint e1.disjoint_gb] at h
+  have := e1.num_clamp y
+  omega
+num_1 := by intros y; rw [e1.num_1, ← Finset.mem_union, ← Finset.mem_union, h₉]
+num_infty := e1.num_infty
+valid_gray := by intros; apply e1.valid_gray; simp_all
+valid_black := by intros _ h
+                  simp at h
+                  cases h
+                  . subst x
+                    tauto
+                  . apply e1.valid_black; assumption
+disjoint_gb := disjoint_gb
+color := by intros a b h₁ h₂
+            rw [← Finset.mem_union, h₉]
+            simp at h₂
+            cases h₂
+            . apply p₃
+              rw [DirectedGraph.edge_succ]
+              subst a
+              assumption
+            . rw [Finset.mem_union]
+              apply e1.color <;> assumption
+stack_finset := by
+  intros y
+  rw [e1.stack_finset]
+  have h : y = x \/ ¬ y = x := by tauto
+  cases h <;> constructor <;> simp_all
+  intros h
+  rw [union_helper] at h
+  apply not_x_in_black
+  simp_all
+  obtain ⟨cc, h, h₁⟩ := h
+  rw [e1.sccs_in_black] at h₁
+  tauto
+simplelist_stack := e1.simplelist_stack
+decreasing_stack := e1.decreasing_stack
+wf_stack₂ := e1.wf_stack₂
+wf_stack₃ := by intros y hy
+                obtain ⟨z, _, _, _⟩ := e1.wf_stack₃ y hy
+                have h₃ : x = z \/ ¬ x = z := by tauto
+                cases h₃
+                . subst z
+                  obtain ⟨z, _, _, ⟨_, _⟩⟩ := h₆
+                  use z
+                  simp
+                  repeat any_goals apply And.intro
+                  any_goals omega
+                  any_goals tauto
+                  . intros h
+                    subst z
+                    omega
+                  . apply reachable_trans _ y x z <;> assumption
+                . use z
+                  simp_all
+                  tauto
+sccs_in_black := by intros cc
+                    rw [e1.sccs_in_black cc]
+                    constructor <;> intros h₁ <;> simp_all <;> intros y h
+                    . simp
+                      right
+                      tauto
+                    . obtain ⟨_, h₁, _⟩ := h₁
+                      have h₄ := h₁ h
+                      simp at h₄
+                      have h₃ : x = y \/ ¬ x = y := by tauto
+                      cases h₃ <;> cases h₄
+                      any_goals subst y
+                      any_goals tauto
+                      exfalso
+                      obtain ⟨y, _, _, _⟩ := h₆
+                      have h := scc_max graph x y cc (by assumption) (by assumption) (by assumption)
+                      specialize h₁ h
+                      simp at h₁
+                      cases h₁
+                      . subst y
+                        simp_all
+                      . have hg : {y} ≤ e1.gray := by simp; assumption
+                        have hb : {y} ≤ e1.black := by simp; assumption
+                        have h := e1.disjoint_gb hg hb
+                        simp at h
+sccs_disjoint := e1.sccs_disjoint
+          }
+
+    p₁ := {
+            eq_gray := by simp
+                          rw [<- p₁.eq_gray]
+                          simp [add_stack_incr]
+                          rw [Finset.erase_eq_of_not_mem]
+                          all_goals tauto
+            sub_black := by simp
+                            have h := p₁.sub_black
+                            simp [add_stack_incr] at h
+                            intros y hy
+                            specialize h hy
+                            simp
+                            tauto
+            sub_sccs := by simp
+                           have h := p₁.sub_sccs
+                           simp [add_stack_incr] at h
+                           assumption
+            stack_num := by simp
+                            have h := p₁.stack_num
+                            simp [add_stack_incr] at h
+                            obtain ⟨_, h⟩ := h
+                            intros y hy
+                            specialize h y hy
+                            split at h
+                            any_goals assumption
+                            subst y
+                            rw [e.stack_finset] at hy
+                            simp at hy
+                            cases hy <;> tauto
+            sub_stack := by simp
+                            use (s ++ [x])
+                            simp_all
+                            intros y h
+                            cases h <;> tauto
+          }
+    p₃ := by simp
+    p₄ := by simp; rw [h₈]; omega
+    p₅ := by right
+             obtain ⟨y, h₁, z, h₂, h₃, h₄⟩ := p₅
+             use z
+             rw [DirectedGraph.edge_succ] at h₁
+             have := DirectedGraph.valid_edge _ _ _ h₁
+             simp_all
+             apply reachable_trans _ x y z <;> tauto
+    p₆ := by simp
+             intros y hy s hs z hz _
+             have hxz : z = x \/ ¬ z = x := by tauto
+             cases hxz
+             . subst z
+               apply p₄
+               rw [DirectedGraph.edge_succ]
+               assumption
+             . apply p₆
+               all_goals simp [add_stack_incr]
+               any_goals tauto
+               obtain ⟨s5, h₃, _⟩ := p₁.sub_stack
+               simp [add_stack_incr] at h₃
+               use s5
+               constructor
+               . tauto
+               . use z
+                 rw [hs, ← singleton_append, ← List.append_assoc] at h₃
+                 have := append_inj_left' h₃ rfl
+                 subst s
+                 simp_all
+  }
+else
+  have disjoint_s2_s3: ∀ x, x ∈ s -> x ∈ e.stack -> False := by
+    intros y h₁ h₂
+    have h := e1.simplelist_stack y
+    obtain ⟨h₇, _⟩ := h₇
+    rw [<- h₇] at h
+    simp [num_occ] at h
+    rw [mem_num_occ] at *
+    split at h
+    all_goals omega
+  {
+    n := (DirectedGraph.vertices graph: List V).length
+    e' := {
+            black := insert x e1.black
+            gray := e.gray
+            stack := e.stack
+            sccs := (toFinset (x :: s)) :: e1.sccs
+            -- sn := e1.sn
+            num := fun (y: V) => if (x :: s).contains y then (DirectedGraph.vertices graph: List V).length else e1.num y
+            num_clamp := by simp
+                            intros y
+                            rw [Finset.card_insert_of_not_mem]
+                            any_goals assumption
+                            split
+                            any_goals tauto
+                            have h := e1.num_clamp y
+                            rw [← p₁.eq_gray] at h
+                            simp [add_stack_incr] at h
+                            rw [Finset.card_insert_of_not_mem] at h
+                            any_goals tauto
+                            cases h <;> omega
+            num_1 := by simp
+                        intros y
+                        split
+                        any_goals simp
+                        any_goals tauto
+                        rw [e1.num_1]
+                        rw [← p₁.eq_gray]
+                        simp [add_stack_incr]
+                        all_goals tauto
+            num_infty := by simp
+                            intros y
+                            rw [e1.num_infty]
+                            have h : (y = x \/ y ∈ s) \/ (¬ (y = x \/ y ∈ s)) := by tauto
+                            cases h <;> constructor
+                            any_goals simp_all
+                            . use (Insert.insert x (toFinset s))
+                              simp
+                              tauto
+                            . intros cc _ _
+                              use cc
+                              tauto
+                            . intros cc hy h
+                              cases h with
+                              | inl h => subst cc
+                                         simp at hy
+                                         tauto
+                              | inr h => tauto
+            valid_gray  := e.valid_gray
+            valid_black := by intros _ h
+                              simp at h
+                              cases h
+                              . subst x
+                                tauto
+                              . apply e1.valid_black; assumption
+            disjoint_gb := by simp
+                              constructor
+                              . assumption
+                              . have h := e1.disjoint_gb
+                                rw [<- p₁.eq_gray] at h
+                                simp [add_stack_incr] at h
+                                tauto
+            color := by intros a b h₁ h₂
+                        simp at h₂
+                        simp
+                        cases h₂ with
+                        | inl h₂ => subst a
+                                    rw [← DirectedGraph.edge_succ] at h₁
+                                    specialize p₃ b h₁
+                                    simp at p₃
+                                    rw [← p₁.eq_gray] at p₃
+                                    simp [add_stack_incr] at p₃
+                                    tauto
+                        | inr h₂ => have h := e1.color a b h₁ h₂
+                                    rw [← p₁.eq_gray] at h
+                                    simp [add_stack_incr] at h
+                                    tauto
+            stack_finset := by obtain ⟨h₇, _⟩ := h₇
+                               rw [tepid e1, ← h₇, ← p₁.eq_gray]
+                               simp [add_stack_incr]
+                               rw [pertinent (Insert.insert x (toFinset s))]
+                               simp
+                               intros y
+                               rw [e.stack_finset]
+                               simp
+                               constructor <;> intros h <;> cases h
+                               any_goals tauto
+                               right
+                               rename_i h
+                               obtain ⟨h₂, h₃⟩:= h
+                               repeat any_goals apply And.intro
+                               . right
+                                 constructor
+                                 . right
+                                   tauto
+                                 . intros h
+                                   cases h
+                                   . subst y; tauto
+                                   . have hg : {y} ≤ e.gray := by simp; assumption
+                                     have hb : {y} ≤ e.black := by simp; assumption
+                                     have h := e.disjoint_gb hg hb
+                                     simp at h
+                               . intros h
+                                 cases h with
+                                 | inl h => subst y; tauto
+                                 | inr h =>
+                                cases (stack_or_scc y (by tauto)) with
+                                | inl h₁ => cases h with
+                                            | inl h => apply disjoint_s2_s3 <;> assumption
+                                            | inr h => rw [union_helper, ← e1.num_infty] at h
+                                                       have h₁ : y ∈ e1.stack := by rw [← h₇]; simp; tauto
+                                                       rw [← stack_num] at h₁
+                                                       omega
+                                | inr h₁ => rw [← union_helper] at h₁
+                                            tauto
+            simplelist_stack := e.simplelist_stack
+            decreasing_stack := by have h := e.decreasing_stack
+                                   simp [Sorted] at h
+                                   simp [Sorted]
+                                   rw [<- List.Pairwise.iff_of_mem]
+                                   . exact h
+                                   . intros a b sa sb
+                                     obtain ⟨h₇, _⟩ := h₇
+                                     have ha := e1.simplelist_stack a
+                                     have hb := e1.simplelist_stack b
+                                     rw [<- h₇] at ha hb
+                                     simp [num_occ] at ha hb
+                                     split <;> split
+                                     any_goals rw [mem_num_occ] at *
+                                     any_goals rename_i h₁ h₂
+                                     any_goals cases h₁
+                                     any_goals cases h₂
+                                     any_goals split at ha
+                                     any_goals split at hb
+                                     any_goals subst a
+                                     any_goals subst b
+                                     any_goals tauto
+                                     any_goals omega
+                                     rw [← mem_num_occ] at *
+                                     rw [← p₁.stack_num, ← p₁.stack_num]
+                                     all_goals simp [add_stack_incr]
+                                     any_goals split
+                                     all_goals tauto
+            wf_stack₂ := by simp
+                            intros a sa b sb h
+                            obtain ⟨h₇, _⟩ := h₇
+                            have := disjoint_s2_s3 a
+                            have := disjoint_s2_s3 b
+                            any_goals split at h
+                            any_goals split at h
+                            all_goals rename_i ha hb
+                            any_goals cases ha
+                            any_goals cases hb
+                            any_goals subst a
+                            any_goals subst b
+                            any_goals tauto
+                            any_goals apply e1.wf_stack₂
+                            any_goals tauto
+                            any_goals rw [<- h₇]
+                            all_goals simp
+                            all_goals tauto
+            wf_stack₃ := by intros y hy
+                            obtain ⟨z, hz, _, _⟩ := e.wf_stack₃ y hy
+                            use z
+                            repeat any_goals apply And.intro
+                            any_goals tauto
+                            any_goals simp
+                            any_goals split
+                            any_goals split
+                            any_goals omega
+                            any_goals apply num_bound
+                            all_goals rename_i hz hy
+                            . cases hz
+                              . subst z
+                                tauto
+                              . exfalso
+                                apply disjoint_s2_s3 z
+                                any_goals assumption
+                                apply gray_le_stack
+                                assumption
+                            . rw [← p₁.stack_num, ← p₁.stack_num]
+                              any_goals simp [add_stack_incr]
+                              any_goals tauto
+                              . split <;> split
+                                any_goals omega
+                                all_goals tauto
+                              . right
+                                apply gray_le_stack
+                                assumption
+            sccs_in_black := by obtain ⟨h₇, s_in_black⟩ := h₇
+                                have h := e1.decreasing_stack
+                                simp [Sorted] at h
+                                rw [← h₇, List.pairwise_append, List.pairwise_cons] at h
+                                obtain ⟨h₆, ⟨h₅, h₈⟩, h₉⟩ := h
+                                have h : ∀ y ∈ s, reachable graph y x := by
+                                  intros y hy
+                                  obtain ⟨z, hz, _, ryz⟩ := e1.wf_stack₃ y (by rw [← h₇]; simp; tauto)
+                                  rw [← p₁.eq_gray] at hz
+                                  simp [add_stack_incr] at hz
+                                  cases hz
+                                  . subst z
+                                    tauto
+                                  . apply reachable_trans graph y z x ryz
+                                    apply e1.wf_stack₂
+                                    any_goals rw [← h₇]
+                                    any_goals simp
+                                    . right; right
+                                      apply gray_le_stack
+                                      assumption
+                                    . apply h₅
+                                      apply gray_le_stack
+                                      assumption
+                                have : is_subscc graph (toFinset (x :: s)) := by
+                                  apply scc_navel x
+                                  . intros y hy
+                                    simp at hy
+                                    cases hy
+                                    . subst y; tauto
+                                    . apply h; tauto
+                                  . intros y hy
+                                    simp at hy
+                                    apply e1.wf_stack₂
+                                    any_goals rw [← h₇]
+                                    any_goals simp
+                                    any_goals tauto
+                                    cases hy
+                                    . subst y; omega
+                                    . apply h₉
+                                      any_goals assumption
+                                      all_goals tauto
+                                have h₄ : ∀ y ∈ (x :: s), ∀ z ∈ e.stack, DirectedGraph.edge graph y z → False := by
+                                  intros y hy z hz y2z
+                                  specialize h₅ z hz
+                                  specialize p₆ z (by tauto)
+                                  simp at p₆
+                                  have := sn_bound e
+                                  have h := e.num_clamp z
+                                  have h₁ := p₁.stack_num z (by tauto)
+                                  simp [add_stack_incr] at h₁
+                                  split at h₁
+                                  any_goals subst z
+                                  any_goals tauto
+                                  rw [← stack_num] at hz
+                                  cases h <;> cases hy
+                                  any_goals omega
+                                  . rw [← DirectedGraph.edge_succ] at y2z
+                                    have := p₄ z y2z
+                                    omega
+                                  . specialize p₆ s (by tauto) y (by tauto) y2z
+                                    omega
+                                have h₅ : ∀ y ∈ (x :: s), ∀ z, DirectedGraph.edge graph y z → z ∈ (e1.gray ∪ e1.black) := by
+                                  intros y hy z hz
+                                  cases hy
+                                  . apply p₃
+                                    rw [DirectedGraph.edge_succ]
+                                    tauto
+                                  . simp
+                                    apply e1.color
+                                    . tauto
+                                    . apply s_in_black
+                                      tauto
+                                have h₁ : ∀ y ∈ (x :: s), ∀ z ∈ e1.sccs.foldl Union.union ∅, in_same_scc graph y z → False := by
+                                  intros y hy z hz h₁
+                                  rw [union_helper] at hz
+                                  obtain ⟨cc, h₁, h₂⟩ := hz
+                                  have : y ∈ cc := by apply scc_max graph z y cc
+                                                      any_goals assumption
+                                                      . rw [e1.sccs_in_black] at h₂
+                                                        tauto
+                                                      . simp [in_same_scc] at *; tauto
+                                  have : e1.num y = (DirectedGraph.vertices graph: List V).length := by
+                                    rw [e1.num_infty]
+                                    use cc
+                                  have h : y ∈ e1.stack := by
+                                    rw [← h₇]
+                                    simp
+                                    simp at hy
+                                    tauto
+                                  rw [← stack_num] at h
+                                  omega
+                                have h : ∀ z, ∀ y ∈ (x :: s), DirectedGraph.edge graph y z → reachable graph z y → z ∈ (x :: s) := by
+                                  intros z y hy y2z z2y
+                                  have h := h₅ y hy z y2z
+                                  rw [stature] at h
+                                  simp at h
+                                  cases h with
+                                  | inl h => rw [← h₇] at h
+                                             simp at h
+                                             cases h with
+                                             | inl h => tauto
+                                             | inr h => cases h with
+                                                        | inl h => subst z; tauto
+                                                        | inr h => exfalso
+                                                                   apply h₄ y (by tauto) z (by tauto) y2z
+                                  | inr h => exfalso
+                                             apply h₁ y hy z h
+                                             constructor
+                                             any_goals assumption
+                                             all_goals tauto
+                                have h₃ : ∀ z, ∀ l₁, ∀ y ∈ (x :: s), path graph y l₁ z → reachable graph z y → z ∈ (x :: s) := by
+                                  intros z l₁
+                                  induction l₁ <;> intros y hy y2z z2y
+                                  . cases y2z
+                                    apply h z y hy
+                                    all_goals assumption
+                                  . rename_i induction_step
+                                    cases y2z
+                                    rename_i head tail h₈ h₉
+                                    have : reachable graph head y := by
+                                      apply reachable_trans _ _ z _
+                                      any_goals assumption
+                                      all_goals tauto
+                                    apply induction_step head
+                                    any_goals tauto
+                                    . apply reachable_trans _ _ y _
+                                      any_goals assumption
+                                      all_goals tauto
+                                have : is_scc graph (toFinset (x :: s)) := by
+                                  constructor
+                                  . assumption
+                                  . intros s' h₂ h₁
+                                    have h : s' ⊆ (toFinset (x :: s)) \/ ¬ s' ⊆ (toFinset (x :: s)) := by tauto
+                                    cases h with
+                                    | inl _ => assumption
+                                    | inr h => exfalso
+                                               simp [Subset] at h
+                                               obtain ⟨z, _, h⟩ := h
+                                               specialize h₁ z x (by assumption) (by apply h₂; simp)
+                                               obtain ⟨h₁, h₂⟩ := h₁
+                                               cases h₂ with
+                                               | inl h₂ => apply h
+                                                           obtain ⟨l, h₂⟩ := h₂
+                                                           specialize h₃ z l x (by tauto) (by assumption) (by assumption)
+                                                           simp at h₃
+                                                           tauto
+                                               | inr h₂ => obtain ⟨_, _⟩ := h₂
+                                                           subst z
+                                                           tauto
+                                intros cc
+                                constructor <;> intros h
+                                . cases h
+                                  all_goals rename_i h
+                                  . apply And.intro
+                                    . use x
+                                      simp
+                                    . apply And.intro
+                                      . simp
+                                        apply Finset.insert_subset_insert
+                                        intros y
+                                        simp
+                                        apply s_in_black
+                                      . tauto
+                                  . have h : cc ∈ e1.sccs := by tauto
+                                    rw [e1.sccs_in_black] at h
+                                    obtain ⟨_, h, _⟩ := h
+                                    any_goals apply And.intro
+                                    any_goals assumption
+                                    any_goals apply And.intro
+                                    any_goals tauto
+                                    . apply Finset.Subset.trans h
+                                      apply Finset.subset_insert
+                                . have h : x ∈ cc \/ ¬ x ∈ cc := by tauto
+                                  cases h
+                                  . have : cc = toFinset (x :: s) := by
+                                      apply disjoint_scc graph
+                                      any_goals assumption
+                                      any_goals tauto
+                                      use x
+                                      simp_all
+                                    subst cc
+                                    tauto
+                                  . obtain ⟨_, h, _⟩ := h
+                                    simp
+                                    right
+                                    rw [e1.sccs_in_black]
+                                    any_goals apply And.intro
+                                    any_goals assumption
+                                    any_goals apply And.intro
+                                    any_goals tauto
+                                    . intros y hy
+                                      specialize h hy
+                                      simp at h
+                                      cases h
+                                      any_goals tauto
+                                      any_goals subst y
+                                      all_goals tauto
+            sccs_disjoint := by intros cc₁ h₁ cc₂ h₂
+                                cases h₁ <;> cases h₂
+                                any_goals tauto
+                                all_goals rename_i h₁ h₂
+                                . right
+                                  rw [eq_empty_iff_forall_not_mem]
+                                  intros z h₆
+                                  simp [*] at h₆
+                                  obtain ⟨h₆, h₈⟩ := h₆
+                                  obtain ⟨h₇, _⟩ := h₇
+                                  have h : z ∈ e1.stack := by rw [← h₇]; cases h₆ <;> simp <;> tauto
+                                  rw [← stack_num] at h
+                                  obtain ⟨_, h⟩ := h
+                                  apply h
+                                  rw [e1.num_infty]
+                                  use cc₂
+                                  tauto
+                                . right
+                                  rw [eq_empty_iff_forall_not_mem]
+                                  intros z h₆
+                                  simp [*] at h₆
+                                  obtain ⟨h₆, h₈⟩ := h₆
+                                  obtain ⟨h₇, _⟩ := h₇
+                                  have h : z ∈ e1.stack := by rw [← h₇]; cases h₈ <;> simp <;> tauto
+                                  rw [← stack_num] at h
+                                  obtain ⟨_, h⟩ := h
+                                  apply h
+                                  rw [e1.num_infty]
+                                  use cc₁
+                                  tauto
+                                . apply e1.sccs_disjoint <;> tauto
+          }
+    p₁ := {
+            eq_gray := by simp
+            sub_black := by simp
+                            intros y hy
+                            have h := p₁.sub_black
+                            simp [add_stack_incr] at h
+                            specialize h hy
+                            simp
+                            tauto
+            sub_sccs := by simp
+                           intros cc h
+                           simp
+                           right
+                           apply p₁.sub_sccs
+                           simp [add_stack_incr]
+                           assumption
+            stack_num := by simp
+                            intros y h
+                            rw [← p₁.stack_num]
+                            any_goals simp [add_stack_incr]
+                            any_goals split
+                            any_goals split
+                            any_goals subst y
+                            any_goals tauto
+                            all_goals rename_i h₁
+                            obtain ⟨h₇, _⟩ := h₇
+                            have h := e1.simplelist_stack y
+                            rw [<- h₇] at h
+                            simp [num_occ] at h
+                            cases h₁
+                            all_goals split at h
+                            any_goals subst y
+                            any_goals rw [mem_num_occ] at *
+                            all_goals omega
+            sub_stack := by simp
+          }
+    p₃ := by simp
+    p₄ := by simp
+    p₅ := by simp
+    p₆ := by simp
+  }
+termination_by (Finset.card (((toFinset (DirectedGraph.vertices graph : List V)) \ (e.gray ∪ e.black)) : Finset V), 0)
+
+
+def dfs [DirectedGraph V Graph]
+        [BEq V] [LawfulBEq V] [DecidableEq V]
+        (graph : Graph) (roots: List V) (e : Env V graph)
+        (a₁ : roots ⊆ DirectedGraph.vertices graph)
+        (a₂ : ∀ x, x ∈ roots -> access_to graph e.gray x)
+        : Shuttle graph roots e := match roots with
+| [] => {
+           n := (DirectedGraph.vertices graph: List V).length
+           e' := e
+           p₁ := {
+                    eq_gray := rfl
+                    sub_black := by tauto
+                    sub_sccs := by tauto
+                    stack_num := by tauto
+                    sub_stack := by use []
+                                    simp_all
+                 }
+           p₃ := by intros; tauto
+           p₄ := by intros; tauto
+           p₅ := by intros; tauto
+           p₆ := by intros _ _ h
+                    obtain ⟨s2, h₁, ⟨x, h₃, _⟩⟩ := h
+                    symm at h₁
+                    rw [List.append_left_eq_self] at h₁
+                    subst s2
+                    tauto
+        }
+| x :: roots =>
+  if dite: (e.num x) == -1 then
+    have h : ¬ x ∈ e.gray ∪ e.black := by intros h
+                                          simp at h
+                                          rw [<- e.num_1] at h
+                                          simp_all
+    let ⟨n1, e1, p₁, p₃, p₄, p₅, pₕ⟩ := dfs3 graph x e (by tauto) (by apply a₂; tauto) (by intros _; apply h; simp_all) (by intros _; apply h; simp_all)
+    have h₂ := by obtain ⟨h, _, _⟩ := p₁
+                  rw [<- h]
+                  intros
+                  apply a₂
+                  tauto
+
+    have t₁ : e.gray ∪ e.black ⊆ toFinset (DirectedGraph.vertices graph) := by
+      intros y h
+      simp at h
+      cases h <;> simp_all
+      . apply e.valid_gray; assumption
+      . apply e.valid_black; assumption
+
+    have t₂ : e1.gray ∪ e1.black ⊆ toFinset (DirectedGraph.vertices graph) := by
+      intros y h
+      simp at h
+      cases h <;> simp_all
+      . apply e1.valid_gray; assumption
+      . apply e1.valid_black; assumption
+
+    have termination_proof : (toFinset (DirectedGraph.vertices graph) \ (e1.gray ∪ e1.black)).card < (toFinset (DirectedGraph.vertices graph) \ (e.gray ∪ e.black)).card := by
+      rw [Finset.card_sdiff]
+      rw [Finset.card_sdiff]
+      any_goals assumption
+      have t₁ := Finset.card_le_card t₁
+      have t₂ := Finset.card_le_card t₂
+      rw [Finset.card_union_of_disjoint e.disjoint_gb] at *
+      rw [Finset.card_union_of_disjoint e1.disjoint_gb] at *
+      obtain ⟨p₁, p₂, _⟩:= p₁
+      rw [p₁] at t₁
+      rw [p₁]
+      have h : e.black ⊂ e1.black := by
+        constructor
+        . exact p₂
+        . intros h₃
+          specialize h₃ p₃
+          apply h
+          simp
+          tauto
+      have h := Finset.card_lt_card h
+      simp_all
+      omega
+
+    let ⟨n2, e2, p₆, p₈, p₉, pₐ, p⟩ := dfs graph roots e1 (by tauto) h₂
+    {
+      n :=  min n1 n2
+      e' := e2
+      p₁ := subenv_trans p₁ p₆
+      p₃ := by intros _ h
+               cases h
+               . simp [Union.union]
+                 right
+                 obtain ⟨_, p₆, _, _, _⟩ := p₆
+                 apply p₆
+                 assumption
+               . tauto
+      p₄ := by intros y h
+               cases h
+               . cases (stack_or_scc x (by tauto)) with
+                 | inl h => obtain ⟨_, _, _, p₆, _⟩ := p₆
+                            specialize p₆ x h
+                            rw [p₆] at p₄
+                            simp_all
+                 | inr h => obtain ⟨cc, h₁, h₂⟩ := h
+                            obtain ⟨_, _, p₆, _, _⟩ := p₆
+                            specialize p₆ h₂
+                            have h : e2.num x = (DirectedGraph.vertices graph: List V).length := by
+                              rw [e2.num_infty]
+                              use cc
+                            rw [h]
+                            cases pₐ <;> try omega
+                            rename_i h
+                            obtain ⟨x, _, _, _, h, _⟩ := h
+                            simp
+                            right
+                            rw [h]
+                            apply num_bound
+               . rename_i h
+                 specialize p₉ y h
+                 omega
+      p₅ := by have h : min n1 n2 = n1 \/ min n1 n2 = n2 := by omega
+               cases h
+               all_goals rename_i h
+               all_goals rw [h]
+               all_goals cases pₐ
+               any_goals tauto
+               all_goals cases p₅
+               any_goals tauto
+               any_goals right
+               . use x
+                 constructor
+                 . tauto
+                 . apply subenv_num_of_reachable <;> assumption
+               . use x
+                 constructor
+                 . tauto
+                 . apply subenv_num_of_reachable <;> assumption
+               . rename_i h _
+                 obtain ⟨y, h⟩ := h
+                 use y
+                 tauto
+               . rename_i h _
+                 obtain ⟨y, h⟩ := h
+                 use y
+                 tauto
+      p₆ := by obtain ⟨_, _, _,  _, ⟨l₁, p₁, _⟩⟩ := p₁
+               obtain ⟨_, _, _, q₂, ⟨l₂, p₆, _⟩⟩ := p₆
+               intros y h h₁
+               specialize p y
+               specialize pₕ y
+               obtain ⟨s2, h₁, ⟨x, h₂, h₃⟩⟩ := h₁
+               rw [p₁, p₆] at *
+               rw [<- List.append_assoc] at h₁
+               have h₁ := List.append_inj_left' h₁ rfl
+               subst s2
+               specialize q₂ y (by simp; tauto)
+               simp at h₂
+               cases h₂
+               . specialize p (by simp; tauto) ⟨l₂, (by tauto), x, (by assumption), (by assumption)⟩
+                 omega
+               . specialize pₕ (by tauto) ⟨l₁, (by tauto), x, (by assumption), (by assumption)⟩
+                 rw [q₂] at *
+                 simp_all
+    }
+  else
+    let ⟨n2, e2, p₁, p₃, p₄, p₅, p₆⟩ := dfs graph roots e (by tauto) (by intros; apply a₂; tauto)
+    have gray_or_black : x ∈ e.gray \/ x ∈ e.black := by
+      rw [<- (e.num_1 x)]
+      simp_all
+    {
+      n := min (e.num x) n2
+      e' := e2
+      p₁ := p₁
+      p₃ := by intros _ h
+               cases h
+               . obtain ⟨h, _, _⟩ := p₁
+                 rw [<- h]
+                 simp
+                 cases gray_or_black <;> tauto
+               . apply p₃; assumption
+      p₄ := by intros y h
+               obtain ⟨_, _, p₇, p₈, _⟩ := p₁
+               cases h <;> rename_i h
+               . cases (stack_or_scc x gray_or_black) <;> rename_i h
+                 . rw [(p₈ _ h)]
+                   simp [*]
+                 . have h₁ : e2.num x = (DirectedGraph.vertices graph: List V).length := by
+                    rw [e2.num_infty]
+                    tauto
+                   rw [h₁]
+                   have : e.num x ≤ (DirectedGraph.vertices graph: List V).length := by apply num_bound
+                   omega
+               . specialize p₄ y h
+                 omega
+      p₅ := by
+              intros
+              have h : n2 ≤ e.num x \/ e.num x < n2 := by omega
+              cases h <;> simp [*] <;> cases p₅
+              any_goals tauto
+              all_goals have : e.num x ≤ n2 := by omega
+              all_goals simp [*]
+              all_goals have h : e.num x = (DirectedGraph.vertices graph: List V).length \/ ¬ e.num x = (DirectedGraph.vertices graph: List V).length := by tauto
+              all_goals cases h
+              any_goals tauto
+              any_goals omega
+              all_goals right; left; use x
+              all_goals have h : x ∈ e.stack := by rw [<- stack_num]; simp_all
+              all_goals have h : e.num x = e2.num x := by obtain ⟨_, _, _, p₁, _⟩ := p₁; apply p₁ _ h
+              all_goals rename_i h₁ h₂ h₃ h₄ h₅
+              all_goals rw [h] at *
+              repeat any_goals apply And.intro
+              any_goals tauto
+              . obtain ⟨_, _, _, _, ⟨s, p₁, _⟩⟩ := p₁
+                rw [p₁]
+                simp
+                tauto
+              . have : e2.num x ≤ (DirectedGraph.vertices graph: List V).length := by apply num_bound
+                simp_all
+              . obtain ⟨_, _, _, _, ⟨s, p₁, _⟩⟩ := p₁
+                rw [p₁]
+                simp_all
+      p₆ := by intros y hy h
+               specialize p₆ y hy h
+               omega
+    }
+termination_by (Finset.card (((toFinset (DirectedGraph.vertices graph : List V)) \ (e.gray ∪ e.black)) : Finset V), roots.length)
+
+end
