kosaraju-lean4/Tarjan/Env.lean
@@ -1,0 +1,411 @@
+import Graph.DirectedGraph
+import Graph.Scc
+import ListHelper.Simplelist
+import ListHelper.Union
+import Mathlib.Data.Finset.Basic
+import Mathlib.Data.Finset.Card
+import Mathlib.Data.List.Sort
+
+open Finset
+open Finset List
+
+structure Env (V : Type*) {Graph : Type*}
+              [BEq V] [LawfulBEq V] [DecidableEq V]
+              [DirectedGraph V Graph]
+              (graph : Graph)
+where
+  black: Finset V
+  gray: Finset V
+  stack: List V
+  sccs: List (Finset V)
+  num:  V -> Int
+  num_clamp : ∀ x, (-1 ≤ num x /\ num x < gray.card + black.card) \/ num x = (DirectedGraph.vertices graph: List V).length
+  num_1 : ∀ x, ¬ num x = (-1) ↔ x ∈ gray \/ x ∈ black
+  num_infty : ∀ x, num x = (DirectedGraph.vertices graph: List V).length ↔ ∃ cc, x ∈ cc /\ cc ∈ sccs
+  valid_gray  : ∀ x ∈ gray,  x ∈ DirectedGraph.vertices graph
+  valid_black : ∀ x ∈ black, x ∈ DirectedGraph.vertices graph
+  disjoint_gb : Disjoint gray black
+  color : no_black_to_white graph black gray
+  stack_finset : ∀ x, x ∈ stack ↔ x ∈ (gray ∪ (black \ sccs.foldl Union.union ∅))
+  simplelist_stack : simplelist stack
+  decreasing_stack : List.Sorted (fun x y => num x ≥ num y) stack
+  -- ∀ x ∈ stack, ∀ y ∈ stack, num x ≤ num y ↔ precedes y x stack
+  wf_stack₂ : ∀ x ∈ stack, ∀ y ∈ stack, num x ≤ num y → reachable graph x y
+  wf_stack₃ : ∀ y ∈ stack, ∃ x ∈ gray,  num x ≤ num y /\ reachable graph y x
+  sccs_in_black : ∀ cc, cc ∈ sccs ↔ Nonempty cc /\ cc ⊆ black /\ is_scc graph cc
+  sccs_disjoint : ∀ cc₁ ∈ sccs, ∀ cc₂ ∈ sccs, cc₁ = cc₂ \/ cc₁ ∩ cc₂ = ∅
+
+structure SubEnv {V Graph : Type*}
+                 [BEq V] [LawfulBEq V] [DecidableEq V]
+                 [DirectedGraph V Graph]
+                 {graph : Graph}
+                 (e e': Env V graph)
+where
+  eq_gray : e.gray = e'.gray
+  sub_black : e.black ⊆ e'.black
+  sub_sccs : e.sccs ⊆ e'.sccs
+  stack_num : ∀ x ∈ e.stack, e.num x = e'.num x
+  sub_stack : ∃ s, e'.stack = s ++ e.stack /\ ∀ x ∈ s, x ∈ e'.black
+
+def subenv_trans [DirectedGraph V Graph]
+                 [BEq V] [LawfulBEq V] [DecidableEq V]
+                 {graph : Graph}
+                 {e1 e2 e3: Env V graph}
+                 (h12 : SubEnv e1 e2)
+                 (h23 : SubEnv e2 e3)
+                 : SubEnv e1 e3 :=
+{
+  eq_gray := by rw [h12.eq_gray, h23.eq_gray]
+  sub_black := Finset.Subset.trans h12.sub_black h23.sub_black
+  sub_sccs := List.Subset.trans h12.sub_sccs h23.sub_sccs
+  stack_num := by intros x h
+                  rw [h12.stack_num x h]
+                  apply h23.stack_num
+                  obtain ⟨s, h, _⟩ := h12.sub_stack
+                  rw [h]
+                  simp
+                  tauto
+  sub_stack := by obtain ⟨l₁, h₁, h₂⟩ := h12.sub_stack
+                  obtain ⟨l₂, h₃, h₄⟩ := h23.sub_stack
+                  use (l₂ ++ l₁)
+                  simp_all
+                  intros x h
+                  cases h with
+                  | inl _ => tauto
+                  | inr h => apply h23.sub_black
+                             apply h₂ _ h
+}
+
+
+def num_of_reachable [DirectedGraph V Graph]
+                     [BEq V] [LawfulBEq V] [DecidableEq V]
+                     {graph : Graph}
+                     (n: Int) (x: V) (e: Env V graph) : Prop :=
+∃ y ∈ e.stack, n = e.num y /\ reachable graph x y
+
+theorem subenv_num_of_reachable
+          [DirectedGraph V Graph]
+          [BEq V] [LawfulBEq V] [DecidableEq V]
+          {graph : Graph}
+          {e e' : Env V graph}
+          {x : V}
+          {n : Int}
+          (h : SubEnv e e') :
+(num_of_reachable n x e) -> num_of_reachable n x e' := by
+simp [num_of_reachable]
+intros x _ _ _
+use x
+obtain ⟨_, _, _, h, ⟨s, h₂⟩⟩ := h
+simp_all
+
+theorem stack_or_scc [DirectedGraph V Graph]
+                     [BEq V] [LawfulBEq V] [DecidableEq V]
+                     {graph : Graph}
+                     {e : Env V graph}
+                     (x : V)
+                     (h₁ : x ∈ e.gray \/ x ∈ e.black) :
+x ∈ e.stack \/ (∃ cc, x ∈ cc /\ cc ∈ e.sccs) := by
+have h₂ : x ∈ List.foldl Union.union ∅ e.sccs \/ ¬ x ∈ List.foldl Union.union ∅ e.sccs := by tauto
+cases h₂
+. right
+  rename_i h
+  rw [union_helper] at h
+  assumption
+. left
+  rw [e.stack_finset]
+  simp
+  tauto
+
+theorem gray_le_stack [DirectedGraph V Graph]
+                     [BEq V] [LawfulBEq V] [DecidableEq V]
+                     {graph : Graph}
+                     {e : Env V graph}
+                     {x : V}
+                     (h₁ : x ∈ e.gray) : x ∈ e.stack := by
+cases (stack_or_scc x (by tauto)) with
+| inl h => tauto
+| inr h => obtain ⟨cc, h, h₁⟩ := h
+           rw [e.sccs_in_black] at h₁
+           obtain ⟨_, h₁, _⟩ := h₁
+           specialize h₁ h
+           have hb : {x} ≤ e.black := by simp; assumption
+           have hg : {x} ≤ e.gray := by simp; assumption
+           have h := e.disjoint_gb hg hb
+           simp at h
+
+theorem barrel [DirectedGraph V Graph]
+               [BEq V] [LawfulBEq V] [DecidableEq V]
+               {graph : Graph}
+               {e : Env V graph} :
+Finset.toList (e.gray ∪ e.black) ⊆ (DirectedGraph.vertices graph: List V) := by
+intro x h₁
+simp_all
+cases h₁
+. apply e.valid_gray; assumption
+. apply e.valid_black; assumption
+
+theorem croissant [DirectedGraph V Graph]
+              [BEq V] [LawfulBEq V] [DecidableEq V]
+              {graph : Graph}
+              (e : Env V graph) :
+(Finset.toList (e.gray ∪ e.black)).length ≤ (DirectedGraph.vertices graph: List V).length := by
+apply List.Subperm.length_le
+apply List.subperm_of_subset
+. apply Finset.nodup_toList
+. apply barrel
+
+theorem shrewd [DirectedGraph V Graph]
+              [BEq V] [LawfulBEq V] [DecidableEq V]
+              {graph : Graph}
+              (e : Env V graph) :
+e.gray ⊔ e.black = toFinset e.stack ⊔ e.sccs.foldl Union.union ∅ := by
+apply Subset.antisymm
+. intros x
+  simp
+  intros h
+  cases h
+  . left
+    apply gray_le_stack
+    assumption
+  . have h₁ : x ∈ e.sccs.foldl Union.union ∅ \/ ¬ x ∈ e.sccs.foldl Union.union ∅ := by tauto
+    cases h₁
+    . tauto
+    . rw [e.stack_finset]
+      simp
+      tauto
+. intros x
+  simp
+  rw [e.stack_finset]
+  simp
+  intros h
+  cases h with
+  | inl h => cases h <;> tauto
+  | inr h => right
+             rw [union_helper] at h
+             obtain ⟨cc, _, h⟩ := h
+             rw [e.sccs_in_black] at h
+             tauto
+
+theorem stature [DirectedGraph V Graph]
+              [BEq V] [LawfulBEq V] [DecidableEq V]
+              {graph : Graph}
+              (e : Env V graph) :
+e.gray ∪ e.black = toFinset e.stack ∪ e.sccs.foldl Union.union ∅ := by
+have h := shrewd e
+simp at h
+tauto
+
+theorem tepid [DirectedGraph V Graph]
+              [BEq V] [LawfulBEq V] [DecidableEq V]
+              {graph : Graph}
+              (e : Env V graph) :
+e.black = (toFinset e.stack ⊔ e.sccs.foldl Union.union ∅) \ e.gray := by
+rw [← shrewd, Disjoint.sup_sdiff_cancel_left]
+exact e.disjoint_gb
+
+theorem sn_bound [DirectedGraph V Graph]
+                 [BEq V] [LawfulBEq V] [DecidableEq V]
+                 {graph : Graph}
+                 (e : Env V graph) :
+e.gray.card + e.black.card ≤ (DirectedGraph.vertices graph: List V).length := by
+have h₁ := croissant e
+simp at h₁
+rw [Finset.card_union_of_disjoint e.disjoint_gb] at h₁
+omega
+
+theorem num_bound [DirectedGraph V Graph]
+                    [BEq V] [LawfulBEq V] [DecidableEq V]
+                    {graph : Graph}
+                    (e : Env V graph)
+                    {x : V} :
+e.num x ≤ (DirectedGraph.vertices graph: List V).length := by
+have := sn_bound e
+cases (e.num_clamp x) <;> omega
+
+theorem stack_num [DirectedGraph V Graph]
+                 [BEq V] [LawfulBEq V] [DecidableEq V]
+                 {graph : Graph}
+                 (e : Env V graph)
+                 (x : V) :
+(¬ e.num x = -1) /\ (¬ e.num x = (DirectedGraph.vertices graph: List V).length) ↔ x ∈ e.stack := by
+rw [e.stack_finset]
+simp
+have h₆ := not_congr (e.num_infty x)
+rw [(e.num_1 x), h₆, <- union_helper]
+constructor
+. tauto
+. intros h
+  cases h with
+  | inl h =>
+    constructor
+    . tauto
+    . intros h₁
+      rw [union_helper] at h₁
+      obtain ⟨cc, h₁, h₃⟩ := h₁
+      have hg : {x} ≤ e.gray := by simp; assumption
+      have hb : {x} ≤ e.black := by simp
+                                    rw [e.sccs_in_black] at h₃
+                                    tauto
+      have h := e.disjoint_gb hg hb
+      simp at h
+  | inr _ => tauto
+
+def add_stack_incr [DirectedGraph V Graph]
+                   [BEq V] [LawfulBEq V] [DecidableEq V]
+                   {graph : Graph}
+                   (e : Env V graph)
+                   (x : V)
+                   (a₁ : x ∈ DirectedGraph.vertices graph)
+                   (a₂ : access_to graph e.gray x)
+                   (a₃ : ¬ x ∈ e.gray)
+                   (a₄ : ¬ x ∈ e.black)
+                   : Env V graph :=
+{
+  gray  := insert x e.gray
+  black := e.black
+  stack := x :: e.stack
+  sccs := e.sccs
+  num   := fun y => if y = x then e.gray.card + e.black.card else e.num y
+--  sn    := e.sn + 1
+  num_clamp := by simp; intros y
+                  rw [Finset.card_insert_of_not_mem a₃]
+                  split
+                  . omega
+                  . cases (e.num_clamp y) <;> omega
+  num_1 := by simp
+              intros y
+              constructor <;> intros h
+              . split at h
+                . tauto
+                . rw [e.num_1] at h
+                  tauto
+              . split
+                . omega
+                . rw [e.num_1]
+                  tauto
+  num_infty := by simp
+                  intros y
+                  split
+                  . subst y
+                    rw [<-(e.num_infty x)]
+                    constructor <;> intros <;> exfalso
+                    . have : (e.gray ∪ e.black) ⊆ (toFinset (DirectedGraph.vertices graph)) := by
+                        intros x h
+                        have := e.valid_gray x
+                        have := e.valid_black x
+                        rw [List.mem_toFinset]
+                        simp at h
+                        cases h <;> tauto
+                      have h : e.gray.card + e.black.card = (DirectedGraph.vertices graph : List V).length := by omega
+                      have : (toFinset (DirectedGraph.vertices graph : List V)).card ≤ (e.gray ∪ e.black).card := by
+                        rw [Finset.card_union_of_disjoint e.disjoint_gb, h]
+                        apply List.toFinset_card_le
+                      have h₁ : e.gray ∪ e.black = toFinset (DirectedGraph.vertices graph) := by apply Finset.eq_of_subset_of_card_le <;> assumption
+                      have h : x ∈ toFinset (DirectedGraph.vertices graph) := by simp; assumption
+                      rw [<- h₁] at h
+                      simp at h
+                      tauto
+                    . have h : ¬ e.num x = -1 := by omega
+                      rw [e.num_1] at h
+                      tauto
+                  . exact e.num_infty y
+  valid_gray  := by intros _ h
+                    simp at h
+                    cases h
+                    . subst x; tauto
+                    . apply e.valid_gray; assumption
+  valid_black := e.valid_black
+  disjoint_gb := by simp_all; exact e.disjoint_gb
+  color := by intros a b h h₁
+              cases (e.color a b h h₁) <;> simp <;> tauto
+  stack_finset := by intros y
+                     simp
+                     rw [e.stack_finset]
+                     simp
+  simplelist_stack := by rw [simplelist_tl]
+                         constructor
+                         . exact e.simplelist_stack
+                         . intros h
+                           rw [e.stack_finset] at h
+                           simp at h
+                           tauto
+  decreasing_stack := by
+                  simp
+                  repeat any_goals apply And.intro
+                  all_goals intros
+                  any_goals split
+                  any_goals subst x
+                  repeat any_goals apply And.intro
+                  any_goals intros
+                  repeat any_goals apply And.intro
+                  any_goals omega
+                  all_goals rename_i y h₂ h₃
+                  . have := e.num_clamp y
+                    rw [<- stack_num] at h₂
+                    omega
+                  . have : ¬ x ∈ e.stack := by
+                      intros h
+                      rw [e.stack_finset] at h
+                      simp at h
+                      tauto
+                    simp [Sorted]
+                    rw [<- List.Pairwise.iff_of_mem]
+                    . exact e.decreasing_stack
+                    . intros a b ha hb
+                      split <;> split
+                      any_goals subst a
+                      any_goals subst b
+                      any_goals tauto
+  wf_stack₂ := by simp
+                  repeat any_goals apply And.intro
+                  any_goals tauto
+                  all_goals intros
+                  repeat any_goals apply And.intro
+                  any_goals intros
+                  all_goals rename_i h
+                  any_goals split at h
+                  any_goals split at h
+                  any_goals subst x
+                  any_goals tauto
+                  all_goals rename_i h₁ y h₃ h₄
+                  . rw [<- stack_num] at h₃
+                    have := e.num_clamp y
+                    omega
+                  . obtain ⟨z, h, _, h₂⟩:= e.wf_stack₃ y h₃
+                    specialize a₂ z h
+                    apply reachable_trans _ y z x <;> tauto
+                  . rw [e.stack_finset] at h₁; simp at h₁; tauto
+                  . rw [e.stack_finset] at h₃; simp at h₃; tauto
+                  . apply e.wf_stack₂ <;> assumption
+  wf_stack₃ := by intro y h
+                  cases h <;> simp_all
+                  . left; tauto
+                  . split
+                    . subst y
+                      exfalso
+                      have h : x ∈ e.stack := by tauto
+                      rw [e.stack_finset] at h
+                      simp at h
+                      tauto
+                    . obtain ⟨z, h⟩ := e.wf_stack₃ y (by tauto)
+                      right
+                      use z
+                      split
+                      . subst z
+                        tauto
+                      . tauto
+  sccs_in_black := e.sccs_in_black
+  sccs_disjoint := e.sccs_disjoint
+}
+
+/-
+def add_black [DirectedGraph V Graph]
+              [BEq V] [LawfulBEq V] [DecidableEq V]
+              {graph : Graph}
+              (x : V)
+              (e : Env V graph) : Env V graph :=
+{
+  e with black := insert x e.black
+         gray  := erase  e.gray x
+}
+-/
