kosaraju-lean4/lakefile.lean
@@ -7,6 +7,8 @@ package «kosaraju» where
 @[default_target]
 lean_lib «Kosaraju» where
   -- add library configuration options here
+lean_lib «Tarjan» where
+lean_lib «ListHelper» where
+lean_lib «Graph» where
 
 require mathlib from git "https://github.com/leanprover-community/mathlib4.git" @ "master"
-
